StmtRel.thy
@@ -635,8 +635,15 @@ lemma exhale_stmt_rel:
           \<comment>\<open>Since the well-definedness must be differentiated from the evaluation state during the exhale,
             there is potentially a step in the Boogie program that sets this differentiation up resulting a new
             relation that tracks both states (where in the beginning both states are the same)\<close>
-      and R_to_Rexh: "red_ast_bpl_rel (uncurry_eq R) (uncurry Rexh) P ctxt \<gamma> \<gamma>1"
-      and ExhaleRel: "exhale_rel Rexh Q ctxt_vpr StateCons P ctxt A \<gamma>1 \<gamma>2"
+\<comment>\<open>      and R_to_Rexh: "red_ast_bpl_rel (uncurry_eq R) (uncurry Rexh) P ctxt \<gamma> \<gamma>1"\<close>
+      \<comment>\<open>The following premise shows the advantage of allowing different input and output relations for
+         \<^term>\<open>exhale_rel\<close>. It allows abstracting over any potential setup code that is required for 
+         encoding an exhale. Note that if we only allowed the same input and output relation, then
+         one would need an additional premise that allows setting up state. This would not only add
+         clutter but also would reduce expressivity because the rule would force an encoding to
+         always set up the state before continuing. As a result, one would not be able to, for example,
+         justify the encoding \<open>if(*) { exhale A; assume false}\<close>.\<close>
+      and ExhaleRel: "exhale_rel (rel_ext_eq R) Rexh Q ctxt_vpr StateCons P ctxt A \<gamma> \<gamma>2"
       and InvHolds: "\<And> \<omega> ns. R \<omega> ns \<Longrightarrow> Q A \<omega> \<omega>"
           \<comment>\<open>At the end of the exhale we require the Boogie program to establish the output relation on the 
              evaluation state\<close>
@@ -655,9 +662,9 @@ lemma exhale_stmt_rel:
 proof (rule stmt_rel_intro)
   fix \<omega> ns \<omega>'
   assume "R \<omega> ns" 
-  with R_to_Rexh obtain ns1 where Red1: "red_ast_bpl P ctxt (\<gamma>, Normal ns) (\<gamma>1, Normal ns1)" and "Rexh \<omega> \<omega> ns1"
+  \<comment>\<open>with R_to_Rexh obtain ns1 where Red1: "red_ast_bpl P ctxt (\<gamma>, Normal ns) (\<gamma>1, Normal ns1)" and "Rexh \<omega> \<omega> ns1"
     unfolding red_ast_bpl_rel_def
-    by auto
+    by auto\<close>
     
   assume RedExhale: "red_stmt_total ctxt_vpr StateCons \<Lambda>_vpr (Exhale A) \<omega> (RNormal \<omega>')"
   hence "StateCons \<omega>'"
@@ -668,10 +675,11 @@ proof (rule stmt_rel_intro)
                         \<exists>ns'. red_ast_bpl P ctxt (\<gamma>, Normal ns) (\<gamma>', Normal ns') \<and> R_out \<omega>' ns'"
   proof cases
     case (RedExhale \<omega>_exh)
-    with exhale_rel_normal_elim[OF ExhaleRel \<open>Rexh \<omega> \<omega> ns1\<close>] obtain ns2 where 
+    with exhale_rel_normal_elim[OF ExhaleRel] \<open>R \<omega> ns\<close> obtain ns2 where 
       "red_ast_bpl P ctxt (\<gamma>, Normal ns) (\<gamma>2, Normal ns2)" and "Rexh \<omega> \<omega>_exh ns2"
-      using red_ast_bpl_transitive[OF Red1] InvHolds[OF \<open>R \<omega> ns\<close>]
+      using InvHolds[OF \<open>R \<omega> ns\<close>]
       by blast
+      
     moreover from rel_success_elim[OF UpdHavoc, where ?\<omega> = "(\<omega>,\<omega>_exh)" and ?\<omega>'="(\<omega>',\<omega>')"] RedExhale \<open>Rexh \<omega> \<omega>_exh ns2\<close> obtain ns3 where
     \<comment>\<open>moreover from Rexh_to_R \<open>Rexh \<omega> \<omega>_exh ns2\<close> obtain ns3 where
       "red_ast_bpl P ctxt (\<gamma>2, Normal ns2) (\<gamma>3, Normal ns3)" and "R_out \<omega>_exh ns3"
@@ -686,16 +694,13 @@ proof (rule stmt_rel_intro)
 next
   fix \<omega> ns \<omega>'
   assume "R \<omega> ns" 
-  with R_to_Rexh obtain ns1 where Red1: "red_ast_bpl P ctxt (\<gamma>, Normal ns) (\<gamma>1, Normal ns1)" and "Rexh \<omega> \<omega> ns1"
-    unfolding red_ast_bpl_rel_def
-    by auto
 
   assume "red_stmt_total ctxt_vpr StateCons \<Lambda>_vpr (Exhale A) \<omega> RFailure"
   thus "\<exists>c'. snd c' = Failure \<and> red_ast_bpl P ctxt (\<gamma>, Normal ns) c'"
   proof cases
     case RedExhaleFailure
-    with exhale_rel_failure_elim[OF ExhaleRel \<open>Rexh \<omega> \<omega> ns1\<close>] show ?thesis
-      using red_ast_bpl_transitive[OF Red1] InvHolds[OF \<open>R \<omega> ns\<close>]
+    with exhale_rel_failure_elim[OF ExhaleRel] \<open>R \<omega> ns\<close> show ?thesis
+      using InvHolds[OF \<open>R \<omega> ns\<close>]
       by fastforce
   qed (simp)
 qed
@@ -709,8 +714,8 @@ lemma exhale_stmt_rel_inst:
       and Consistent: "\<And> \<omega> ns. R \<omega> ns \<Longrightarrow> StateCons \<omega>"    
       and InvHolds: "\<And> \<omega> ns. R \<omega> ns \<Longrightarrow> Q A \<omega> \<omega>"
       \<comment>\<open>and "\<And> \<omega> ns. R \<omega> ns \<Longrightarrow> \<exists>ns'. red_ast_bpl P ctxt (\<gamma>, Normal ns) (\<gamma>1, Normal ns') \<and> (state_rel Pr StateCons TyRep Tr' AuxPred' ctxt \<omega> \<omega> ns')"\<close>
-      and R_to_Rexh: "red_ast_bpl_rel R (state_rel_def_same Pr StateCons TyRep Tr' AuxPred' ctxt) P ctxt \<gamma> \<gamma>1"
-      and ExhRel: "exhale_rel (state_rel Pr StateCons TyRep Tr' AuxPred' ctxt) Q ctxt_vpr StateCons P ctxt A \<gamma>1 \<gamma>2"
+\<comment>\<open>      and R_to_Rexh: "red_ast_bpl_rel R (state_rel_def_same Pr StateCons TyRep Tr' AuxPred' ctxt) P ctxt \<gamma> \<gamma>1"\<close>
+      and ExhRel: "exhale_rel (rel_ext_eq R) (state_rel Pr StateCons TyRep Tr' AuxPred' ctxt) Q ctxt_vpr StateCons P ctxt A \<gamma> \<gamma>2"
       (*and "\<And> \<omega>def \<omega> ns. (state_rel Pr StateCons TyRep Tr' AuxPred' ctxt) \<omega>def \<omega> ns \<Longrightarrow> 
                       \<exists>ns'. red_ast_bpl P ctxt (\<gamma>2, Normal ns) (\<gamma>3, Normal ns') \<and> R_out \<omega> ns'"*)
       \<comment>\<open>and Rexh_to_Rout: "red_ast_bpl_rel (uncurry (state_rel Pr StateCons TyRep Tr' AuxPred' ctxt))  (\<lambda>\<omega>def_\<omega> ns. R_out (snd \<omega>def_\<omega>) ns) P ctxt \<gamma>2 \<gamma>3"
@@ -725,12 +730,8 @@ lemma exhale_stmt_rel_inst:
                 ) (\<lambda>_. False) P ctxt \<gamma>2 \<gamma>'"
     shows "stmt_rel R R_out ctxt_vpr StateCons \<Lambda>_vpr P ctxt (Exhale A) \<gamma> \<gamma>'"
 proof (rule exhale_stmt_rel[OF WfConsistency])
-  show "red_ast_bpl_rel (uncurry_eq R) (uncurry (state_rel Pr StateCons TyRep Tr' AuxPred' ctxt)) P ctxt \<gamma> \<gamma>1"
-    using R_to_Rexh
-    unfolding red_ast_bpl_rel_def
-    by simp
-next
-  show "exhale_rel (state_rel Pr StateCons TyRep Tr' AuxPred' ctxt) Q ctxt_vpr StateCons P ctxt A \<gamma>1 \<gamma>2"
+
+  show "exhale_rel (rel_ext_eq R) (state_rel Pr StateCons TyRep Tr' AuxPred' ctxt) Q ctxt_vpr StateCons P ctxt A \<gamma> \<gamma>2"
     by (rule ExhRel) 
 (*
 next
@@ -760,8 +761,8 @@ lemma exhale_stmt_rel_inst_no_inv:
   assumes WfConsistency: "wf_total_consistency ctxt_vpr StateCons StateCons_t"
       and Consistent: "\<And> \<omega> ns. R \<omega> ns \<Longrightarrow> StateCons \<omega>"
       and InvHolds: "\<And> \<omega> ns. R \<omega> ns \<Longrightarrow> True" \<comment>\<open>not required, but makes proof generation uniform (same number of premises for each case)\<close>
-      and R_to_Rexh: "red_ast_bpl_rel R (state_rel_def_same Pr StateCons TyRep Tr' AuxPred' ctxt) P ctxt \<gamma> \<gamma>1"
-      and "exhale_rel (state_rel Pr StateCons TyRep Tr' AuxPred' ctxt) (\<lambda>_ _ _. True) ctxt_vpr StateCons P ctxt A \<gamma>1 \<gamma>2"
+      \<comment>\<open>and R_to_Rexh: "red_ast_bpl_rel R (state_rel_def_same Pr StateCons TyRep Tr' AuxPred' ctxt) P ctxt \<gamma> \<gamma>1"\<close>
+      and "exhale_rel (rel_ext_eq R) (state_rel Pr StateCons TyRep Tr' AuxPred' ctxt) (\<lambda>_ _ _. True) ctxt_vpr StateCons P ctxt A \<gamma> \<gamma>2"
     \<comment>\<open>  and Rexh_to_Rout: "red_ast_bpl_rel (uncurry (state_rel Pr StateCons TyRep Tr' AuxPred' ctxt))  (\<lambda>\<omega>def_\<omega> ns. R (snd \<omega>def_\<omega>) ns) P ctxt \<gamma>2 \<gamma>3"
       and "\<And> \<omega> \<omega>' ns. R \<omega> ns \<Longrightarrow> StateCons \<omega>' \<Longrightarrow> \<omega>' \<in> exhale_state ctxt_vpr \<omega> (get_mh_total_full \<omega>) \<Longrightarrow>
                              \<exists>ns'. red_ast_bpl P ctxt (\<gamma>3, Normal ns) (\<gamma>', Normal ns') \<and> R \<omega>' ns'" \<close>
@@ -780,8 +781,8 @@ lemma exhale_stmt_rel_inst_framing_inv:
   assumes WfConsistency: "wf_total_consistency ctxt_vpr StateCons StateCons_t"
       and StateRelAndConsistent: "\<And> \<omega> ns. R \<omega> ns \<Longrightarrow> state_rel_def_same Pr StateCons TyRep Tr AuxPred ctxt \<omega> ns \<and> StateCons \<omega>"
       and InvHolds: "\<And> \<omega> ns. R \<omega> ns \<Longrightarrow> framing_exh ctxt_vpr StateCons A \<omega> \<omega>"
-      and R_to_Rexh: "red_ast_bpl_rel R (state_rel_def_same Pr StateCons TyRep Tr' AuxPred' ctxt) P ctxt \<gamma> \<gamma>1"
-      and ExhRel: "exhale_rel (state_rel Pr StateCons TyRep Tr' AuxPred' ctxt) (framing_exh ctxt_vpr StateCons) ctxt_vpr StateCons P ctxt A \<gamma>1 \<gamma>2"
+      \<comment>\<open>and R_to_Rexh: "red_ast_bpl_rel R (state_rel_def_same Pr StateCons TyRep Tr' AuxPred' ctxt) P ctxt \<gamma> \<gamma>1"\<close>
+      and ExhRel: "exhale_rel (rel_ext_eq R) (state_rel Pr StateCons TyRep Tr' AuxPred' ctxt) (framing_exh ctxt_vpr StateCons) ctxt_vpr StateCons P ctxt A \<gamma> \<gamma>2"
     \<comment>\<open>  and Rexh_to_Rout: "red_ast_bpl_rel (uncurry (state_rel Pr StateCons TyRep Tr' AuxPred' ctxt))  (\<lambda>\<omega>def_\<omega> ns.  state_rel_def_same Pr StateCons TyRep Tr AuxPred ctxt (snd \<omega>def_\<omega>) ns) P ctxt \<gamma>2 \<gamma>3"
       and "\<And> \<omega> \<omega>' ns. state_rel_def_same Pr StateCons TyRep Tr AuxPred ctxt \<omega> ns \<Longrightarrow> StateCons \<omega>' \<Longrightarrow> \<omega>' \<in> exhale_state ctxt_vpr \<omega> (get_mh_total_full \<omega>) \<Longrightarrow>
                              \<exists>ns'. red_ast_bpl P ctxt (\<gamma>3, Normal ns) (\<gamma>', Normal ns') \<and>  state_rel_def_same Pr StateCons TyRep Tr AuxPred ctxt \<omega>' ns'"\<close>
@@ -794,7 +795,7 @@ lemma exhale_stmt_rel_inst_framing_inv:
                        snd \<omega>' \<in> havoc_locs_state ctxt_vpr (snd \<omega>) ({loc. get_mh_total_full (fst \<omega>) loc > 0 \<and> get_mh_total_full (snd \<omega>) loc = 0})
                 ) (\<lambda>_. False) P ctxt \<gamma>2 \<gamma>'"
     shows "stmt_rel R (state_rel_def_same Pr StateCons TyRep Tr AuxPred ctxt) ctxt_vpr StateCons \<Lambda>_vpr P ctxt (Exhale A) \<gamma> \<gamma>'"
-  apply (rule exhale_stmt_rel_inst[OF WfConsistency _ _ R_to_Rexh ExhRel UpdHavoc])
+  apply (rule exhale_stmt_rel_inst[OF WfConsistency _ _ ExhRel UpdHavoc])
   using assms
   by auto
 
@@ -1068,22 +1069,19 @@ abbreviation state_rel_capture_total_state :: \<comment>\<open>make type explici
                        ctxt"
 
 lemma assert_stmt_rel:
-  assumes CaptureState: "red_ast_bpl_rel (uncurry_eq R) (\<lambda> \<omega> ns. (uncurry (RStore (snd \<omega>))) \<omega> ns) P ctxt \<gamma> \<gamma>1"
-      and InvHolds: "\<And> \<omega> ns. R \<omega> ns \<Longrightarrow> Q A \<omega> \<omega>"
-      and ExhaleRel: "\<And>\<omega>0. exhale_rel (RStore \<omega>0) Q ctxt_vpr StateCons P ctxt A \<gamma>1 \<gamma>2"
+  assumes \<comment>\<open>CaptureState: "red_ast_bpl_rel (uncurry_eq R) (\<lambda> \<omega> ns. (uncurry (RStore (snd \<omega>))) \<omega> ns) P ctxt \<gamma> \<gamma>1"\<close>
+          InvHolds: "\<And> \<omega> ns. R \<omega> ns \<Longrightarrow> Q A \<omega> \<omega>"
+      and ExhaleRel: "\<And>\<omega>0. exhale_rel (rel_ext_eq R) (RStore \<omega>0) Q ctxt_vpr StateCons P ctxt A \<gamma> \<gamma>2"
       and ResetState: "\<And> \<omega>0. rel_general (uncurry (RStore \<omega>0)) (uncurry_eq R) (\<lambda> \<omega>1 \<omega>2. \<omega>2 = (\<omega>0,\<omega>0)) (\<lambda>_. False) P ctxt \<gamma>2 \<gamma>'"
     shows "stmt_rel R R ctxt_vpr StateCons \<Lambda>_vpr P ctxt (ViperLang.Assert A) \<gamma> \<gamma>'"
 proof (rule stmt_rel_intro_2)
   fix \<omega> ns res
   assume "R \<omega> ns" and RedStmt: "red_stmt_total ctxt_vpr StateCons \<Lambda>_vpr (stmt.Assert A) \<omega> res"
 
-  hence "uncurry_eq R (\<omega>,\<omega>) ns"
-    by simp
-
+\<comment>\<open>
   with CaptureState obtain ns1 where RedBplInit: "red_ast_bpl P ctxt (\<gamma>, Normal ns) (\<gamma>1, Normal ns1)" and RStoreInit: "(RStore \<omega>) \<omega> \<omega> ns1"
     unfolding red_ast_bpl_rel_def
-    by auto
-    
+    by auto\<close>    
     
   show "rel_vpr_aux R P ctxt \<gamma> \<gamma>' ns res"
   proof (rule rel_vpr_aux_intro)
@@ -1094,16 +1092,16 @@ proof (rule stmt_rel_intro_2)
       by (auto elim: RedAssertNormal_case)
 
 
-    from this obtain ns_exh where RedBplExh: "red_ast_bpl P ctxt (\<gamma>1, Normal ns1) (\<gamma>2, Normal ns_exh)" and 
+    from this obtain ns_exh where RedBplExh: "red_ast_bpl P ctxt (\<gamma>, Normal ns) (\<gamma>2, Normal ns_exh)" and 
                                   "(RStore \<omega>) \<omega> \<omega>_exh ns_exh" 
-      using exhale_rel_normal_elim[OF ExhaleRel RStoreInit InvHolds[OF \<open>R \<omega> ns\<close>]]
+      using exhale_rel_normal_elim[OF ExhaleRel _ InvHolds[OF \<open>R \<omega> ns\<close>]] \<open>R \<omega> ns\<close>
       by blast
       
     with rel_success_elim[OF ResetState]
     obtain ns' where "red_ast_bpl P ctxt (\<gamma>2, Normal ns_exh) (\<gamma>', Normal ns')" and "R \<omega> ns'"
       by fastforce
 
-    with RedBplInit RedBplExh
+    with RedBplExh
     show "\<exists>ns'. red_ast_bpl P ctxt (\<gamma>, Normal ns) (\<gamma>', Normal ns') \<and> R \<omega>' ns'"
       using \<open>\<omega> = \<omega>'\<close> red_ast_bpl_transitive
       by blast
@@ -1114,8 +1112,7 @@ proof (rule stmt_rel_intro_2)
       by (auto elim: RedAssertFailure_case)
 
     thus "\<exists>c'. red_ast_bpl P ctxt (\<gamma>, Normal ns) c' \<and> snd c' = Failure"
-      using exhale_rel_failure_elim[OF ExhaleRel RStoreInit InvHolds[OF \<open>R \<omega> ns\<close>]]
-            RedBplInit red_ast_bpl_transitive
+      using exhale_rel_failure_elim[OF ExhaleRel _ InvHolds[OF \<open>R \<omega> ns\<close>]] \<open>R \<omega> ns\<close>
       by (metis (no_types, opaque_lifting) snd_conv)
   qed
 qed
@@ -1123,17 +1120,16 @@ qed
 lemma assert_stmt_rel_inst:
   assumes "m = mask_var Tr \<and> h = heap_var Tr"
       and InvHolds: "\<And> \<omega> ns. state_rel_def_same Pr StateCons TyRep Tr AuxPred ctxt \<omega> ns \<Longrightarrow> Q A \<omega> \<omega>"
-      and CaptureState: "red_ast_bpl_rel (uncurry_eq (state_rel_def_same Pr StateCons TyRep Tr AuxPred ctxt))
+     \<comment>\<open> and CaptureState: "red_ast_bpl_rel (uncurry_eq (state_rel_def_same Pr StateCons TyRep Tr AuxPred ctxt))
                            (\<lambda> \<omega> ns. (uncurry (state_rel_capture_total_state Pr StateCons TyRep Tr' AuxPred ctxt m h (snd \<omega>))) \<omega> ns)
-                           P ctxt \<gamma> \<gamma>1"
-      and ExhaleRel: "\<And>\<omega>0. exhale_rel (state_rel_capture_total_state Pr StateCons TyRep Tr' AuxPred ctxt m h \<omega>0) Q ctxt_vpr StateCons P ctxt A \<gamma>1 \<gamma>2"
+                           P ctxt \<gamma> \<gamma>1"\<close>
+      and ExhaleRel: "\<And>\<omega>0. exhale_rel (rel_ext_eq (state_rel_def_same Pr StateCons TyRep Tr AuxPred ctxt)) (state_rel_capture_total_state Pr StateCons TyRep Tr' AuxPred ctxt m h \<omega>0) Q ctxt_vpr StateCons P ctxt A \<gamma> \<gamma>2"
       and ResetState: "\<And> \<omega>0. rel_general (uncurry (state_rel_capture_total_state Pr StateCons TyRep Tr' AuxPred ctxt m h \<omega>0))
                                           (uncurry_eq (state_rel_def_same Pr StateCons TyRep Tr AuxPred ctxt)) 
                                           (\<lambda> \<omega>1 \<omega>2. \<omega>2 = (\<omega>0,\<omega>0)) (\<lambda>_. False) P ctxt \<gamma>2 \<gamma>'"
     shows "stmt_rel (state_rel_def_same Pr StateCons TyRep Tr AuxPred ctxt) (state_rel_def_same Pr StateCons TyRep Tr AuxPred ctxt) ctxt_vpr StateCons \<Lambda>_vpr P ctxt 
                     (ViperLang.Assert A) \<gamma> \<gamma>'"
   apply (rule assert_stmt_rel[where ?RStore = "state_rel_capture_total_state Pr StateCons TyRep Tr' AuxPred ctxt m h", where ?Q=Q])
-     apply (rule CaptureState)
     apply (rule InvHolds)
     apply assumption
    apply (rule ExhaleRel)
@@ -1141,9 +1137,9 @@ lemma assert_stmt_rel_inst:
   done
 
 lemma assert_stmt_rel_alt:
-  assumes CaptureState: "red_ast_bpl_rel (uncurry_eq R) (uncurry Rexh) P ctxt \<gamma> \<gamma>1"
-      and InvHolds: "\<And> \<omega> ns. R \<omega> ns \<Longrightarrow> Q A \<omega> \<omega>"
-      and ExhaleRel: "exhale_rel Rexh Q ctxt_vpr StateCons P ctxt A \<gamma>1 \<gamma>2"
+  assumes \<comment>\<open>CaptureState: "red_ast_bpl_rel (uncurry_eq R) (uncurry Rexh) P ctxt \<gamma> \<gamma>1"\<close>
+          InvHolds: "\<And> \<omega> ns. R \<omega> ns \<Longrightarrow> Q A \<omega> \<omega>"
+      and ExhaleRel: "exhale_rel (rel_ext_eq R) Rexh Q ctxt_vpr StateCons P ctxt A \<gamma> \<gamma>2"
    \<comment>\<open>The second disjunct makes explicit that since the assert has no effect on the Viper state,
       the Boogie encoding can continue from any point that is reachable from \<^term>\<open>\<gamma>\<close>.
       The first disjunct allows the Boogie encoding to reach \<^term>\<open>\<gamma>'\<close> from \<^term>\<open>\<gamma>2\<close> (i.e., the point
@@ -1158,13 +1154,6 @@ lemma assert_stmt_rel_alt:
 proof (rule stmt_rel_intro_2)
   fix \<omega> ns res
   assume "R \<omega> ns" and RedStmt: "red_stmt_total ctxt_vpr StateCons \<Lambda>_vpr (stmt.Assert A) \<omega> res"
-
-  hence "uncurry_eq R (\<omega>,\<omega>) ns"
-    by simp
-
-  with CaptureState obtain ns1 where RedBplInit: "red_ast_bpl P ctxt (\<gamma>, Normal ns) (\<gamma>1, Normal ns1)" and RStoreInit: "Rexh \<omega> \<omega> ns1"
-    unfolding red_ast_bpl_rel_def
-    by auto    
     
   show "rel_vpr_aux R P ctxt \<gamma> \<gamma>' ns res"
   proof (rule rel_vpr_aux_intro)
@@ -1175,9 +1164,9 @@ proof (rule stmt_rel_intro_2)
       by (auto elim: RedAssertNormal_case)
 
 
-    from this obtain ns_exh where RedBplExh: "red_ast_bpl P ctxt (\<gamma>1, Normal ns1) (\<gamma>2, Normal ns_exh)" and 
+    from this obtain ns_exh where RedBplExh: "red_ast_bpl P ctxt (\<gamma>, Normal ns) (\<gamma>2, Normal ns_exh)" and 
                                   "Rexh \<omega> \<omega>_exh ns_exh" 
-      using exhale_rel_normal_elim[OF ExhaleRel RStoreInit InvHolds[OF \<open>R \<omega> ns\<close>]]
+      using exhale_rel_normal_elim[OF ExhaleRel _ InvHolds[OF \<open>R \<omega> ns\<close>]] \<open>R \<omega> ns\<close>
       by blast
 
     from disjE[OF ResetState]
@@ -1187,7 +1176,7 @@ proof (rule stmt_rel_intro_2)
       with \<open>Rexh \<omega> \<omega>_exh ns_exh\<close> rel_success_elim[OF 1]
       obtain ns' where "red_ast_bpl P ctxt (\<gamma>2, Normal ns_exh) (\<gamma>', Normal ns')" and "R \<omega> ns'"
         by fastforce  
-      with RedBplInit RedBplExh
+      with RedBplExh
       show ?thesis
         using \<open>\<omega> = \<omega>'\<close> red_ast_bpl_transitive
         by blast
@@ -1205,8 +1194,7 @@ proof (rule stmt_rel_intro_2)
       by (auto elim: RedAssertFailure_case)
 
     thus "\<exists>c'. red_ast_bpl P ctxt (\<gamma>, Normal ns) c' \<and> snd c' = Failure"
-      using exhale_rel_failure_elim[OF ExhaleRel RStoreInit InvHolds[OF \<open>R \<omega> ns\<close>]]
-            RedBplInit red_ast_bpl_transitive
+      using exhale_rel_failure_elim[OF ExhaleRel _ InvHolds[OF \<open>R \<omega> ns\<close>]] \<open>R \<omega> ns\<close>
       by (metis (no_types, opaque_lifting) snd_conv)
   qed
 qed
